Liveness.v
@@ -2,6 +2,7 @@
 (* Licensing information is available in the LICENSE file. *)
 (* (C) 2020 Nandor Licker. All rights reserved. *)
 
+Require Import Coq.ZArith.ZArith.
 Require Import Coq.Lists.List.
 Require Import LLIR.LLIR.
 Require Import LLIR.Dom.
@@ -11,7 +12,27 @@ Inductive LiveAt: func -> reg -> node -> Prop :=
   | live_at:
     forall
       (f: func) (r: reg) (n: node) (use: node) (p: list node)
-      (PATH: Path f n p use)
-      (NO_DEF: forall (def: node), def <> n -> In def p -> ~DefinedAt f def r)
+      (PATH: ReversePath f n p use)
+      (NO_DEF: forall (def: node), In def (tl p) -> ~DefinedAt f def r)
       (USE: UsedAt f use r),
       LiveAt f r n.
+
+Theorem live_at_succ:
+  forall (f: func) (r: reg) (n: node),
+    LiveAt f r n ->
+    UsedAt f n r
+    \/
+    exists (s: node), SuccOf f n s /\ LiveAt f r s.
+Proof.
+  intros f r n Hlive; inversion Hlive; subst.
+  inversion PATH; subst.
+  { left; auto. }
+  {
+    right; exists next; split; auto.
+    apply live_at with use p0; auto.
+    intros def Hin.
+    destruct p0; [inversion Hin|].
+    simpl in NO_DEF; simpl in Hin.
+    apply NO_DEF; right; assumption.
+  }
+Qed.
