SmallStep.v
@@ -34,7 +34,7 @@ Inductive Normal: prog -> estate -> Prop :=
   | normal_state:
     forall
       (p: prog)
-      (fr_id: positive) (frs: list positive) 
+      (fr_id: positive) (frs: list positive)
       (next: positive) (frames: PTrie.t frame) (init: objects)
       (h: heap)
       (VP: valid_prog p)
@@ -47,13 +47,15 @@ Inductive Final: estate -> Prop :=
   | final_exit:
     forall (stk: PTrie.t frame) (h: heap),
       Final (Exit stk h)
+  | final_broken:
+      Final (Broken)
   .
 
 Inductive Executing: prog -> stack -> frame -> func -> node -> inst -> Prop :=
   | executing:
     forall
       (p: prog)
-      (fr_id: positive) (frs: list positive) 
+      (fr_id: positive) (frs: list positive)
       (next: positive) (frames: PTrie.t frame) (init: objects)
       (f: func) (fr: frame) (i: inst)
       (FRAME: Some fr  = frames ! fr_id)
@@ -70,7 +72,7 @@ Theorem valid_state_can_execute:
 Proof.
   intros p h stk Hvalid.
   inversion Hvalid; inversion FR; inversion VALID.
-  exists fr; exists f; exists (fr_pc fr); exists i.
+  exists fr. exists f. exists (fr_pc fr). exists i.
   apply (executing p fr_id frs next frames init f fr i); auto.
 Qed.
 
@@ -98,11 +100,7 @@ Proof.
   assert (Hlive: LiveAt f r pc).
   {
     apply live_at with (p := [pc]) (use := pc); auto.
-    { apply path_nil; auto. }
-    {
-      intros def Hne Hin.
-      inversion Hin; subst; contradiction.
-    }
+    { apply reverse_path_nil; auto. }
   }
   apply REGS in Hlive.
   destruct Hlive as [v Hreg]; exists v; auto.
@@ -116,16 +114,16 @@ Definition update_frame (stk: stack) (fn: frame -> frame): stack :=
    ; stk_init := stk.(stk_init)
    |}.
 
-Definition set_pc (stk: stack) (pc: node): stack :=
+Definition stk_set_pc (stk: stack) (pc: node): stack :=
   update_frame stk (fun frame => set_pc frame pc).
 
-Definition set_vreg (stk: stack) (r: reg) (v: value): stack :=
+Definition stk_set_vreg (stk: stack) (r: reg) (v: value): stack :=
   update_frame stk (fun frame => set_vreg frame r v).
 
-Definition set_vreg_pc (stk: stack) (r: reg) (v: value) (pc: node): stack :=
+Definition stk_set_vreg_pc (stk: stack) (r: reg) (v: value) (pc: node): stack :=
   update_frame stk (fun frame => set_vreg_pc frame r v pc).
 
-Definition jump_to_phi (stk: stack) (t: node): stack :=
+Definition stk_jump_to_phi (stk: stack) (t: node): stack :=
   update_frame stk (fun frame => jump_to_phi frame t).
 
 Axiom eval_unop: ty -> unop -> value -> option value.
@@ -190,7 +188,7 @@ Inductive BinarySig: value -> value -> binop -> ty -> signal -> Prop :=
   .
 
 Lemma binary_value_or_signal:
-  forall (op: binop) (lhs: value) (rhs: value) 
+  forall (op: binop) (lhs: value) (rhs: value)
     (lhs_ty: ty) (rhs_ty: ty) (dst_ty: ty),
     WellTypedBinop op lhs_ty rhs_ty dst_ty ->
     TypeOfValue lhs lhs_ty ->
@@ -245,7 +243,7 @@ Proof.
 Qed.
 
 Lemma syscall_args:
-  forall 
+  forall
     (p: prog) (f: func)
     (fr: frame) (args: list reg) (env: type_env),
     (Some f = p ! (fr_func fr)) ->
@@ -269,7 +267,7 @@ Proof.
   { intros arg Hin. apply Htyped. right. auto. }
   assert (Hlive': forall arg, In arg args -> LiveAt f arg (fr_pc fr)).
   { intros arg Hin. apply Hlive. right. auto. }
-  generalize (IHargs Htypes' Hlive'); intros [values Hvalues]. 
+  generalize (IHargs Htypes' Hlive'); intros [values Hvalues].
   clear Htypes' Hlive' IHargs.
   assert (Hin: In a (a :: args)). { left; auto. }
   generalize (Hlive a Hin); intros Hlive_a.
@@ -287,7 +285,7 @@ Inductive ReturnToFrame
   : prog ->
     stack ->
     positive ->
-    list positive -> 
+    list positive ->
     inst ->
     node ->
     Prop :=
@@ -295,7 +293,7 @@ Inductive ReturnToFrame
     forall
       (p: prog)
       (next_id: positive)
-      (next: positive) (frames: PTrie.t frame) (init: objects) 
+      (next: positive) (frames: PTrie.t frame) (init: objects)
       (top: positive) (next: positive) (rest: list positive)
       (fr: frame) (f: func) (i: inst) (ret_pc: node)
       (FRAME: Some fr = frames ! next)
@@ -348,7 +346,7 @@ Inductive CallArgs : frame -> list reg -> list value -> Prop :=
   .
 
 Lemma call_args:
-  forall 
+  forall
     (p: prog) (f: func)
     (fr: frame) (args: list reg),
     (Some f = p ! (fr_func fr)) ->
@@ -384,7 +382,7 @@ Inductive step (p: prog): estate -> trace -> estate -> Prop :=
         p
         (State stk h)
         []
-        (State (set_pc stk next) h')
+        (State (stk_set_pc stk next) h')
   | eval_st_sig:
     forall
       (stk: stack) (h: heap) (fr: frame) (f: func) (pc: node)
@@ -423,7 +421,7 @@ Inductive step (p: prog): estate -> trace -> estate -> Prop :=
         p
         (State stk h)
         []
-        (State (set_vreg_pc stk dst dst_value next) h)
+        (State (stk_set_vreg_pc stk dst dst_value next) h)
   | eval_ld_sig:
     forall
       (stk: stack) (h: heap) (fr: frame) (f: func) (pc: node)
@@ -448,7 +446,7 @@ Inductive step (p: prog): estate -> trace -> estate -> Prop :=
         p
         (State stk h)
         []
-        (State (set_vreg_pc stk dst dst_value next) h)
+        (State (stk_set_vreg_pc stk dst dst_value next) h)
   | eval_int:
     forall
       (stk: stack) (h: heap) (fr: frame) (f: func) (pc: node)
@@ -458,7 +456,7 @@ Inductive step (p: prog): estate -> trace -> estate -> Prop :=
         p
         (State stk h)
         []
-        (State (set_vreg_pc stk dst (VInt v) next) h)
+        (State (stk_set_vreg_pc stk dst (VInt v) next) h)
   | eval_select_true:
     forall
       (stk: stack) (h: heap) (fr: frame) (f: func) (pc: node)
@@ -472,7 +470,7 @@ Inductive step (p: prog): estate -> trace -> estate -> Prop :=
         p
         (State stk h)
         []
-        (State (set_vreg_pc stk dst lhs_value next) h)
+        (State (stk_set_vreg_pc stk dst lhs_value next) h)
   | eval_select_false:
     forall
       (stk: stack) (h: heap) (fr: frame) (f: func) (pc: node)
@@ -486,7 +484,7 @@ Inductive step (p: prog): estate -> trace -> estate -> Prop :=
         p
         (State stk h)
         []
-        (State (set_vreg_pc stk dst rhs_value next) h)
+        (State (stk_set_vreg_pc stk dst rhs_value next) h)
   | eval_frame:
     forall
       (stk: stack) (h: heap) (fr: frame) (f: func) (pc: node)
@@ -497,7 +495,7 @@ Inductive step (p: prog): estate -> trace -> estate -> Prop :=
         (State stk h)
         []
         (State
-          (set_vreg_pc stk dst
+          (stk_set_vreg_pc stk dst
             (VSym (SFrame (stk_fr stk) object offset))
             next)
           h)
@@ -512,7 +510,7 @@ Inductive step (p: prog): estate -> trace -> estate -> Prop :=
         (State stk h)
         []
         (State
-          (set_vreg_pc stk dst
+          (stk_set_vreg_pc stk dst
             (VSym (SAtom segment object offset))
             next)
           h)
@@ -525,7 +523,7 @@ Inductive step (p: prog): estate -> trace -> estate -> Prop :=
         p
         (State stk h)
         []
-        (State (set_vreg_pc stk dst (VSym (SFunc fn_id)) next) h)
+        (State (stk_set_vreg_pc stk dst (VSym (SFunc fn_id)) next) h)
   | eval_und:
     forall
       (stk: stack) (h: heap) (fr: frame) (f: func) (pc: node)
@@ -535,7 +533,7 @@ Inductive step (p: prog): estate -> trace -> estate -> Prop :=
         p
         (State stk h)
         []
-        (State (set_vreg_pc stk dst (VUnd) next) h)
+        (State (stk_set_vreg_pc stk dst (VUnd) next) h)
   | eval_jmp:
     forall
       (stk: stack) (h: heap) (fr: frame) (f: func) (pc: node)
@@ -545,13 +543,13 @@ Inductive step (p: prog): estate -> trace -> estate -> Prop :=
         p
         (State stk h)
         []
-        (State (jump_to_phi stk target) h)
+        (State (stk_jump_to_phi stk target) h)
   | eval_jcc_true:
     forall
       (stk: stack) (h: heap) (fr: frame) (f: func) (pc: node)
       (cond: node)
       (brancht: node) (branchf: node)
-      (cond_value: value) 
+      (cond_value: value)
       (EXEC: Executing p stk fr f pc (LLJcc cond brancht branchf))
       (COND: Some cond_value = fr.(fr_regs) ! cond)
       (TRUE: IsTrue cond_value),
@@ -559,7 +557,7 @@ Inductive step (p: prog): estate -> trace -> estate -> Prop :=
         p
         (State stk h)
         []
-        (State (jump_to_phi stk brancht) h)
+        (State (stk_jump_to_phi stk brancht) h)
   | eval_jcc_false:
     forall
       (stk: stack) (h: heap) (fr: frame) (f: func) (pc: node)
@@ -573,7 +571,7 @@ Inductive step (p: prog): estate -> trace -> estate -> Prop :=
         p
         (State stk h)
         []
-        (State (jump_to_phi stk branchf) h)
+        (State (stk_jump_to_phi stk branchf) h)
   | eval_unary_value:
     forall
       (stk: stack) (h: heap) (fr: frame) (f: func) (pc: node)
@@ -586,7 +584,7 @@ Inductive step (p: prog): estate -> trace -> estate -> Prop :=
         p
         (State stk h)
         []
-        (State (set_vreg_pc stk dst dst_value next) h)
+        (State (stk_set_vreg_pc stk dst dst_value next) h)
   | eval_unary_signal:
     forall
       (stk: stack) (h: heap) (fr: frame) (f: func) (pc: node)
@@ -613,7 +611,7 @@ Inductive step (p: prog): estate -> trace -> estate -> Prop :=
         p
         (State stk h)
         []
-        (State (set_vreg_pc stk dst dst_value next) h)
+        (State (stk_set_vreg_pc stk dst dst_value next) h)
   | eval_binary_signal:
     forall
       (stk: stack) (h: heap) (fr: frame) (f: func) (pc: node)
@@ -639,7 +637,7 @@ Inductive step (p: prog): estate -> trace -> estate -> Prop :=
         p
         (State stk h)
         []
-        (State (set_vreg_pc stk dst arg_value next) h)
+        (State (stk_set_vreg_pc stk dst arg_value next) h)
   | eval_syscall_ret:
     forall
       (stk: stack) (h: heap) (fr: frame) (f: func) (pc: node)
@@ -656,7 +654,7 @@ Inductive step (p: prog): estate -> trace -> estate -> Prop :=
         p
         (State stk h)
         tr
-        (State (set_vreg_pc stk' dst (VInt (INT.Int64 dst_value)) next) h')
+        (State (stk_set_vreg_pc stk' dst (VInt (INT.Int64 dst_value)) next) h')
   | eval_syscall_sig:
     forall
       (stk: stack) (h: heap) (fr: frame) (f: func) (pc: node)
@@ -688,7 +686,7 @@ Inductive step (p: prog): estate -> trace -> estate -> Prop :=
         p
         (State stk h)
         tr
-        (State (set_vreg_pc stk dst (VInt (INT.Int64 ENOSYS)) next) h)
+        (State (stk_set_vreg_pc stk dst (VInt (INT.Int64 ENOSYS)) next) h)
   | eval_syscall_und_enosys:
     forall
       (stk: stack) (h: heap) (fr: frame) (f: func) (pc: node)
@@ -703,7 +701,7 @@ Inductive step (p: prog): estate -> trace -> estate -> Prop :=
         p
         (State stk h)
         tr
-        (State (set_vreg_pc stk dst (VInt (INT.Int64 ENOSYS)) next) h)
+        (State (stk_set_vreg_pc stk dst (VInt (INT.Int64 ENOSYS)) next) h)
  | eval_trap:
     forall
       (stk: stack) (h: heap) (fr: frame) (f: func) (pc: node)
@@ -725,9 +723,9 @@ Inductive step (p: prog): estate -> trace -> estate -> Prop :=
         (Signal stk h SIGILL)
   | eval_ret_void:
     forall
-      (stk: stack) (h: heap) 
+      (stk: stack) (h: heap)
       (fr: frame) (f: func) (pc: node) (value: option reg)
-       (rest: list positive) 
+       (rest: list positive)
       (i: inst) (callee: positive) (ret_pc: node)
       (EXEC: Executing p stk fr f pc (LLRet value))
       (NEXT: ReturnToFrame p stk callee rest i ret_pc)
@@ -737,7 +735,7 @@ Inductive step (p: prog): estate -> trace -> estate -> Prop :=
         (State stk h)
         []
         (State
-          (jump_to_phi 
+          (stk_jump_to_phi
             (mkstack
               callee
               rest
@@ -761,8 +759,8 @@ Inductive step (p: prog): estate -> trace -> estate -> Prop :=
         (State stk h)
         []
         (State
-          (jump_to_phi
-            (set_vreg 
+          (stk_jump_to_phi
+            (stk_set_vreg
               (mkstack
                 callee
                 rest
@@ -853,7 +851,7 @@ Inductive step (p: prog): estate -> trace -> estate -> Prop :=
       (stk: stack) (h: heap)
       (stk_fr: positive) (stk_frs: list positive) (stk_next: positive)
       (stk_frames: PTrie.t frame) (stk_init: objects)
-      (fr: frame) (f: func) (pc: node) (callee: reg) 
+      (fr: frame) (f: func) (pc: node) (callee: reg)
       (next: node) (dst: option (ty * reg))
       (callee_func: name) (callee_f: func)
       (args: list reg) (arg_values: list value)
@@ -913,429 +911,6 @@ Inductive step (p: prog): estate -> trace -> estate -> Prop :=
             stk_init)
           h)
   .
-
-Theorem well_typed_progress:
-  forall (p: prog) (st: estate),
-    WellTypedProg p ->
-    valid_prog p ->
-    Normal p st ->
-    ~Final st ->
-    exists (tr: trace) (st': estate),
-      step p st tr st'.
-Proof.
-  intros p st Hwty Hvp Hv Hnf; destruct st.
-  {
-    generalize (valid_state_can_execute p h stk Hv);
-    intros [fr [f [pc [i Hexec]]]]; subst.
-    inversion Hv as [
-        p' stk_fr stk_frs stk_next stk_frames stk_init
-        h' Hvalid Hvalid_top Hvalid_mid Hp' Hstk
-    ]; subst p' h'.
-    inversion Hexec as [
-        p'' stk_fr' stk_frs' stk_next' stk_frames'' stk_init''
-        func' frame' i''
-        FRAME' FUNC' INST' Hp'' Hstk' Hinst Hfunc' Epc Hi''
-    ]; subst i'' func' frame' p''.
-    assert (H_f_valid: valid_func f).
-    { unfold valid_prog in Hvp. apply Hvp with (n := fr_func fr); auto. }
-    assert (Hwtf: WellTypedFunc f).
-    { inversion Hwty; apply FUNCS with (n := fr_func fr); auto. }
-    assert (Hwti: WellTypedInst (ty_env f) i).
-    {
-      inversion Hwtf; inversion INSTS;
-      apply INSTS0 with (n := (fr_pc fr)); auto.
-    }
-    inversion Hvalid_top; inversion VALID; subst fr_id frames p0 p1 fr1.
-    generalize (uses_are_defined p h stk f fr pc i Hv Hexec); intros Hval.
-    rewrite <- Hstk in Hstk'; inversion Hstk'; clear Hstk';
-    subst stk_fr' stk_frs' stk_frames'' stk_init'' stk_next'.
-    rewrite <- FRAME in FRAME'; inversion FRAME'; subst fr0.
-    rewrite <- FUNC in FUNC'; inversion FUNC'; subst f0.
-    rewrite Hstk.
-
-    Ltac used_value f fr pc i sym sym_val Hsym Hreg :=
-      match goal with
-      | [ Hval: forall (r: reg), UsedAt f pc r -> _ |- _ ] =>
-        let H := fresh in
-        assert (H: UsedAt f pc sym);
-        [ constructor; apply inst_used_at with i; subst i pc; auto; constructor
-        |];
-        apply Hval in H;
-        destruct H as [sym_val Hreg];
-        assert (Hsym: Some sym_val = fr.(fr_regs) ! sym);
-        [ rewrite Hreg; reflexivity |]
-      end.
-
-    Ltac step_state :=
-      match goal with
-      | [ |- context [ step _ _ ?tr ?state ] ] => exists tr; exists state; auto
-      end.
-
-    Ltac used_args pc i args0 values Hvalues :=
-      match goal with
-      | [ REGS: context [ LiveAt ?f _ _ -> _ ]
-        , FUNC: Some ?f = ?p ! (fr_func ?fr)
-        |- _ ] =>
-          let H := fresh in
-          assert (H: forall arg, In arg args0 -> LiveAt f arg (fr_pc fr));
-            [ intros arg Hin;
-              apply live_at with (use := pc) (p := [pc]);
-              [ subst pc; constructor; auto
-              | intros def Hne Hin'; inversion Hin'; subst; contradiction
-              | apply used_at_inst; apply inst_used_at with i; subst i pc; 
-                auto; constructor; auto
-              ]
-            |];
-          destruct (call_args p f fr args0 FUNC REGS H) as [values Hvalues]
-      end.
-
-    Ltac used_callee h callee callee_value Hcallee_reg args0 :=
-      match goal with
-      | [ Hexec: Executing ?p ?stk ?fr ?f ?pc ?inst |- _ ] =>
-        destruct (Function_dec callee_value) as [Eq|Ne];
-          [|
-            assert (Hc: Callee inst callee); [constructor|];
-            symmetry in Hcallee_reg;
-            generalize (eval_call_broken 
-              p stk h fr f pc inst callee callee_value
-              Hexec Hc Hcallee_reg Ne
-            ); step_state
-          ]
-      end.
-
-    destruct i eqn:Ei;
-      try match goal with
-      | [ dst: ty * reg |- _ ] => destruct dst as [t dst]
-      end.
-    {
-      used_value f fr pc i addr addr_value Haddr Haddr_reg.
-      destruct (load_value_or_signal stk h t addr_value) as [Hload|Hsig].
-      {
-        destruct Hload as [dst_value Hload].
-        generalize (eval_ld_value
-          p stk h fr f pc dst t next addr
-          addr_value dst_value Hexec Haddr Hload
-        ); step_state.
-      }
-      {
-        destruct Hsig as [sig Hsig].
-        generalize (eval_ld_sig
-          p stk h fr f pc dst t next addr
-          addr_value sig Hexec Haddr Hsig
-        ); step_state.
-      }
-    }
-    {
-      generalize (arg_complete fr index t); intros [dst_value Harg].
-      generalize (eval_arg
-        p stk h fr f pc dst t next index dst_value
-        Hexec Harg
-      ); step_state.
-    }
-    {
-      generalize (eval_int p stk h fr f pc dst next value Hexec).
-      step_state.
-    }
-    {
-      used_value f fr pc i cond cond_value Hcond Hcond_reg.
-      destruct (value_is_true_or_false cond_value) as [Eq|Ne].
-      {
-        used_value f fr pc i vt vt_value Hvt Hvt_reg.
-        generalize (eval_select_true
-          p stk h fr f pc dst t next cond vt vf
-          cond_value vt_value Hexec Hcond Hvt Eq
-        ); step_state.
-      }
-      {
-        used_value f fr pc i vf vf_value Hvf Hvf_reg.
-        generalize (eval_select_false
-          p stk h fr f pc dst t next cond vt vf
-          cond_value vf_value Hexec Hcond Hvf Ne
-        ); step_state.
-      }
-    }
-    {
-      generalize (eval_frame
-        p stk h fr f pc dst next object offset
-        Hexec
-      ); step_state.
-    }
-    {
-      generalize (eval_global
-        p stk h fr f pc dst next segment object offset
-        Hexec
-      ); step_state.
-    }
-    { generalize (eval_func p stk h fr f pc dst next func Hexec); step_state. }
-    { generalize (eval_und p stk h fr f pc t dst next Hexec); step_state. }
-    {
-      used_value f fr pc i arg arg_value Harg Harg_reg.
-      inversion Hwti; subst t0 dst0 next0 op0 arg0.
-      unfold well_typed_reg in ARG_TY;
-      destruct (VALS arg arg_value Harg) as [arg_ty [Harg_ty Harg_type_of]];
-      rewrite ARG_TY in Harg_ty; inversion Harg_ty; subst argt.
-      destruct (unary_value_or_signal op arg_value arg_ty t OP Harg_type_of) as 
-        [ [dst_value [_ Hdst]]
-        | [sig Hsig]
-        ].
-      {
-        generalize (eval_unary_value
-          p stk h fr f pc dst t next op arg dst_value arg_value
-          Hexec Harg Hdst
-        ); step_state.
-      }
-      {
-        generalize (eval_unary_signal
-          p stk h fr f pc dst t next op arg arg_value sig
-          Hexec Harg Hsig
-        ); step_state.
-      }
-    }
-    {
-      used_value f fr pc i lhs lhs_value Hlhs Hlhs_reg.
-      used_value f fr pc i rhs rhs_value Hrhs Hrhs_reg.
-      inversion Hwti; subst t0 dst0 next0 op0 l r.
-      unfold well_typed_reg in LHS_TY;
-      destruct (VALS lhs lhs_value Hlhs) as [lhs_ty [Hlhs_ty Hlhs_type_of]];
-      rewrite LHS_TY in Hlhs_ty; inversion Hlhs_ty; subst tl.
-      unfold well_typed_reg in RHS_TY;
-      destruct (VALS rhs rhs_value Hrhs) as [rhs_ty [Hrhs_ty Hrhs_type_of]];
-      rewrite RHS_TY in Hrhs_ty; inversion Hrhs_ty; subst tr.
-      destruct (binary_value_or_signal 
-        op lhs_value rhs_value lhs_ty rhs_ty t 
-        OP Hlhs_type_of Hrhs_type_of) as [[dst_value [_ Hdst]]|[sig Hsig]].
-      {
-        generalize (eval_binary_value
-          p stk h fr f pc dst t op lhs rhs next lhs_value rhs_value dst_value
-          Hexec Hlhs Hrhs Hdst
-        ); step_state.
-      }
-      {
-        generalize (eval_binary_signal
-          p stk h fr f pc dst t op lhs rhs next lhs_value rhs_value sig
-          Hexec Hlhs Hrhs Hsig
-        ); step_state.
-      }
-    }
-    {
-      used_value f fr pc i src src_value Hsrc Hsrc_reg.
-      generalize (eval_mov
-        p stk h fr f pc dst t next src src_value
-        Hexec Hsrc
-      ); step_state.
-    }
-    {
-      used_value f fr pc i sno sno_value Hsno Hsno_reg.
-      symmetry in Hsno_reg.
-      generalize (VALS sno sno_value Hsno_reg); intros [ty [Hty Hty_of]].
-      inversion Hwti; subst next0 dst0 sno0 args1.
-      unfold well_typed_reg in SNO_TY.
-      rewrite <- Hty in SNO_TY; inversion SNO_TY; subst ty.
-      rename args0 into sys_args.
-      assert (Hargs_live: forall arg, In arg sys_args -> LiveAt f arg (fr_pc fr)).
-      {
-        intros arg Hin'.
-        apply live_at with (use := pc) (p := [pc]).
-        - subst pc; constructor; apply REACH.
-        - intros def contra Hin; inversion Hin; subst; contradiction.
-        - apply used_at_inst; apply inst_used_at with i; subst; try constructor; auto.
-      }
-      generalize (syscall_args 
-        p f fr sys_args (ty_env f)
-        FUNC ARG_TY REGS Hargs_live VALS
-      ); intros [sys_values Hsys_args].
-      destruct (syscall_number_complete sno_value Hty_of) as [[s Esys]|[ENoSys|EUnd]].
-      {
-        destruct (syscall_ret_or_sig s sys_values stk h) as 
-          [ [tr [stk'' [h'' [dst_value Eret]]]]
-          | [sig [tr Esig]]
-          ].
-        {
-          generalize (eval_syscall_ret
-            p stk h fr f pc dst next tr sys_args sys_values sno s sno_value
-            dst_value stk'' h''
-            Hsys_args Hsno_reg Esys Hexec Eret
-          ); step_state.
-        }
-        {
-          generalize (eval_syscall_sig
-            p stk h fr f pc dst next tr sys_args sys_values sno s sno_value sig
-            Hsys_args Hsno_reg Esys Hexec Esig
-          ); step_state.
-        }
-      }
-      {
-        generalize (eval_syscall_nosys
-          p stk h fr f pc dst next [] sys_args sys_values sno sno_value
-          Hsys_args Hsno_reg ENoSys Hexec
-        ); step_state.
-      }
-      {
-        generalize (eval_syscall_und_enosys
-          p stk h fr f pc dst next [] sys_args sys_values sno sno_value
-        ); step_state.
-      }
-    }
-    {
-      used_value f fr pc i callee callee_value Hcallee Hcallee_reg.
-      used_callee h callee callee_value Hcallee_reg args0.
-      used_args pc i args0 values Hvalues.
-      inversion Eq as [func Hfunc]; subst callee_value.
-      generalize (FN_VALS callee func Hcallee); intros Hsome_func.
-      destruct (p ! func) as [callee_fn|] eqn:Efunc; try contradiction.
-      symmetry in Efunc.
-      generalize (eval_call
-        p stk h stk_fr stk_frs stk_next stk_frames stk_init
-        fr f pc callee next dst func callee_fn args0 values
-        Hexec Hcallee Efunc Hvalues
-      ); rewrite Hstk; step_state.
-    }
-    {
-      used_value f fr pc i callee callee_value Hcallee Hcallee_reg.
-      used_callee h callee callee_value Hcallee_reg args0.
-      used_args pc i args0 values Hvalues.
-      inversion Eq as [func Hfunc]; subst callee_value.
-      generalize (FN_VALS callee func Hcallee); intros Hsome_func.
-      destruct (p ! func) as [callee_fn|] eqn:Efunc; try contradiction.
-      symmetry in Efunc.
-      generalize (eval_invoke
-        p stk h stk_fr stk_frs stk_next stk_frames stk_init
-        fr f pc callee next dst exn func callee_fn args0 values
-        Hexec Hcallee Efunc Hvalues
-      ); rewrite Hstk; step_state.
-    }
-    {
-      used_value f fr pc i callee callee_value Hcallee Hcallee_reg.
-      used_callee h callee callee_value Hcallee_reg args0.
-      used_args pc i args0 values Hvalues.
-      inversion Eq as [fn Hfn]. rewrite <- Hfn in Hcallee.
-      generalize (FN_VALS callee fn Hcallee); intros Hfn_not_none.
-      destruct (p ! fn) as [func|] eqn:Efunc; try contradiction.
-      symmetry in Efunc.
-      generalize (eval_tcall 
-        p stk h stk_fr stk_frs stk_next stk_frames stk_init fr f
-        pc callee fn func args0 values Hexec Hcallee Efunc Hvalues).
-      rewrite Hstk.
-      step_state.
-    }
-    {
-      used_value f fr pc i callee callee_value Hcallee Hcallee_reg.
-      used_callee h callee callee_value Hcallee_reg args0.
-      used_args pc i args0 values Hvalues.
-      inversion Eq as [fn Hfn]. rewrite <- Hfn in Hcallee.
-      generalize (FN_VALS callee fn Hcallee); intros Hfn_not_none.
-      destruct (p ! fn) as [func|] eqn:Efunc; try contradiction.
-      symmetry in Efunc.
-      generalize (eval_tinvoke 
-        p stk h stk_fr stk_frs stk_next stk_frames stk_init fr f
-        pc callee exn fn func args0 values Hexec Hcallee Efunc Hvalues).
-      rewrite Hstk.
-      step_state.
-    }
-    {
-      used_value f fr pc i addr addr_value Haddr Haddr_reg.
-      used_value f fr pc i value value_value Hvalue Hvalue_reg.
-      destruct (store_value_signal_break stk h addr_value value_value) as 
-        [ [h'' Evalue]
-        | [ [s Esig]| Ebreak]
-        ].
-      {
-        generalize (eval_st_value
-          p stk h fr f pc next addr value addr_value value_value h''
-          Hexec Haddr Hvalue Evalue
-        ); step_state.
-      }
-      {
-        generalize (eval_st_sig
-          p stk h fr f pc next addr value addr_value s
-          Hexec Haddr Esig
-        ); step_state.
-      }
-      {
-        generalize (eval_st_break 
-          p stk h fr f pc next addr value addr_value
-          Hexec Haddr Ebreak
-        ); step_state.
-      }
-    }
-    {
-      destruct (top_or_return stk) as [Htop|[vr [vrs Hret]]].
-      {
-        generalize (eval_ret_top p stk h fr f pc value Hexec Htop); step_state.
-      }
-      {
-        inversion Hret as [next frames init top ret frs H']; subst ret frs.
-        rewrite <- Hstk in H'; inversion H'; subst top frames init next.
-        assert (Hmvr: In vr stk_frs). { subst; left; auto. }
-        generalize (Hvalid_mid vr Hmvr); intros Hmid.
-        inversion Hmid. subst p0 fr_id frames.
-        rewrite H'; rewrite Hstk.
-        assert (Hret_addr: exists (ret_pc: node), ReturnAddress i1 ret_pc).
-        {
-           destruct RETURN as [H''|[tr [dstr H'']]]; 
-           inversion H''; exists next; constructor.
-        }
-        destruct Hret_addr as [ret_pc Hret_pc].
-        assert (Hret_to_frame: ReturnToFrame p stk vr vrs i1 ret_pc).
-        {
-          subst stk stk_frs; apply return_to_frame with fr0 f0; auto.
-        }
-        destruct RETURN as [Hvoid|[tr [dstr Hcall]]].
-        {
-          generalize (eval_ret_void 
-            p stk h fr f pc value vrs i1 vr ret_pc
-            Hexec Hret_to_frame Hvoid
-          ); step_state.
-        }
-        {
-          assert (Hrv: exists v, ReturnValue fr value tr v).
-          {
-            destruct value as [arg|] eqn:Evalue.
-            {
-              used_value f fr pc i arg arg_value Harg Harg_reg.
-              destruct (TypeOfValue_dec arg_value tr).
-              { exists arg_value; constructor; auto. }
-              { exists VUnd; apply return_some_und with arg_value; auto. }
-            }
-            {
-              exists VUnd; constructor.
-            }
-          }
-          destruct Hrv as [ret_value Hret_value].
-          generalize (eval_ret_value 
-            p stk h fr f pc value vrs i1 vr tr dstr ret_pc ret_value
-            Hexec Hret_to_frame Hcall Hret_value
-          ); step_state.
-        }
-      }
-    }
-    {
-      used_value f fr pc i cond cond_value Hcond Hcond_reg.
-      destruct (value_is_true_or_false cond_value) as [Et|Ef].
-      {
-        generalize (eval_jcc_true 
-          p stk h fr f pc cond bt bf cond_value
-          Hexec Hcond Et
-        ); step_state.
-      }
-      {
-        generalize (eval_jcc_false
-          p stk h fr f pc cond bt bf cond_value
-          Hexec Hcond Ef
-        ); step_state.
-      }
-    }
-    {
-      generalize (eval_jmp p stk h fr f pc target); step_state.
-    }
-    {
-      generalize (eval_trap p stk h fr f pc Hexec); step_state.
-    }
-  }
-  { inversion Hv. }
-  { inversion Hv. }
-  { inversion Hv. }
-Qed.
 
 Inductive star (p: prog): estate -> trace -> estate -> Prop :=
   | star_refl:
