SmallStep_Progress.v
@@ -1,0 +1,448 @@
+(* This file is part of the LLIR Semantics project. *)
+(* Licensing information is available in the LICENSE file. *)
+(* (C) 2020 Nandor Licker. All rights reserved. *)
+
+Require Import Coq.Lists.List.
+Require Import Coq.ZArith.ZArith.
+
+Require Import LLIR.Values.
+Require Import LLIR.Maps.
+Require Import LLIR.LLIR.
+Require Import LLIR.Dom.
+Require Import LLIR.Eval.
+Require Import LLIR.SSA.
+Require Import LLIR.Block.
+Require Import LLIR.Typing.
+Require Import LLIR.Signal.
+Require Import LLIR.Liveness.
+Require Import LLIR.Syscall.
+Require Import LLIR.Frame.
+Require Import LLIR.State.
+Require Import LLIR.SmallStep.
+
+Import ListNotations.
+
+
+
+Theorem small_step_progress:
+  forall (p: prog) (st: estate),
+    WellTypedProg p ->
+    valid_prog p ->
+    Normal p st ->
+    ~Final st ->
+    exists (tr: trace) (st': estate),
+      step p st tr st'.
+Proof.
+  intros p st Hwty Hvp Hv Hnf; destruct st.
+  {
+    generalize (valid_state_can_execute p h stk Hv);
+    intros [fr [f [pc [i Hexec]]]]; subst.
+    inversion Hv as [
+        p' stk_fr stk_frs stk_next stk_frames stk_init
+        h' Hvalid Hvalid_top Hvalid_mid Hp' Hstk
+    ]; subst p' h'.
+    inversion Hexec as [
+        p'' stk_fr' stk_frs' stk_next' stk_frames'' stk_init''
+        func' frame' i''
+        FRAME' FUNC' INST' Hp'' Hstk' Hinst Hfunc' Epc Hi''
+    ]; subst i'' func' frame' p''.
+    assert (H_f_valid: valid_func f).
+    { unfold valid_prog in Hvp. apply Hvp with (n := fr_func fr); auto. }
+    assert (Hwtf: WellTypedFunc f).
+    { inversion Hwty; apply FUNCS with (n := fr_func fr); auto. }
+    assert (Hwti: WellTypedInst (ty_env f) i).
+    {
+      inversion Hwtf; inversion INSTS;
+      apply INSTS0 with (n := (fr_pc fr)); auto.
+    }
+    inversion Hvalid_top; inversion VALID; subst fr_id frames p0 p1 fr1.
+    generalize (uses_are_defined p h stk f fr pc i Hv Hexec); intros Hval.
+    rewrite <- Hstk in Hstk'; inversion Hstk'; clear Hstk';
+    subst stk_fr' stk_frs' stk_frames'' stk_init'' stk_next'.
+    rewrite <- FRAME in FRAME'; inversion FRAME'; subst fr0.
+    rewrite <- FUNC in FUNC'; inversion FUNC'; subst f0.
+    rewrite Hstk.
+
+    Ltac used_value f fr pc i sym sym_val Hsym Hreg :=
+      match goal with
+      | [ Hval: forall (r: reg), UsedAt f pc r -> _ |- _ ] =>
+        let H := fresh in
+        assert (H: UsedAt f pc sym);
+        [ constructor; apply inst_used_at with i; subst i pc; auto; constructor
+        |];
+        apply Hval in H;
+        destruct H as [sym_val Hreg];
+        assert (Hsym: Some sym_val = fr.(fr_regs) ! sym);
+        [ rewrite Hreg; reflexivity |]
+      end.
+
+    Ltac step_state :=
+      match goal with
+      | [ |- context [ step _ _ ?tr ?state ] ] => exists tr; exists state; auto
+      end.
+
+    Ltac used_args pc i args0 values Hvalues :=
+      match goal with
+      | [ REGS: context [ LiveAt ?f _ _ -> _ ]
+        , FUNC: Some ?f = ?p ! (fr_func ?fr)
+        |- _ ] =>
+          let H := fresh in
+          assert (H: forall arg, In arg args0 -> LiveAt f arg (fr_pc fr));
+            [ intros arg Hin;
+              apply live_at with (use := pc) (p := [pc]);
+              [ subst pc; constructor; auto
+              | intros def Hne Hin'; inversion Hin'; subst; contradiction
+              | apply used_at_inst; apply inst_used_at with i; subst i pc;
+                auto; constructor; auto
+              ]
+            |];
+          destruct (call_args p f fr args0 FUNC REGS H) as [values Hvalues]
+      end.
+
+    Ltac used_callee h callee callee_value Hcallee_reg args0 :=
+      match goal with
+      | [ Hexec: Executing ?p ?stk ?fr ?f ?pc ?inst |- _ ] =>
+        destruct (Function_dec callee_value) as [Eq|Ne];
+          [|
+            assert (Hc: Callee inst callee); [constructor|];
+            symmetry in Hcallee_reg;
+            generalize (eval_call_broken
+              p stk h fr f pc inst callee callee_value
+              Hexec Hc Hcallee_reg Ne
+            ); step_state
+          ]
+      end.
+
+    destruct i eqn:Ei;
+      try match goal with
+      | [ dst: ty * reg |- _ ] => destruct dst as [t dst]
+      end.
+    {
+      used_value f fr pc i addr addr_value Haddr Haddr_reg.
+      destruct (load_value_or_signal stk h t addr_value) as [Hload|Hsig].
+      {
+        destruct Hload as [dst_value Hload].
+        generalize (eval_ld_value
+          p stk h fr f pc dst t next addr
+          addr_value dst_value Hexec Haddr Hload
+        ); step_state.
+      }
+      {
+        destruct Hsig as [sig Hsig].
+        generalize (eval_ld_sig
+          p stk h fr f pc dst t next addr
+          addr_value sig Hexec Haddr Hsig
+        ); step_state.
+      }
+    }
+    {
+      generalize (arg_complete fr index t); intros [dst_value Harg].
+      generalize (eval_arg
+        p stk h fr f pc dst t next index dst_value
+        Hexec Harg
+      ); step_state.
+    }
+    {
+      generalize (eval_int p stk h fr f pc dst next value Hexec).
+      step_state.
+    }
+    {
+      used_value f fr pc i cond cond_value Hcond Hcond_reg.
+      destruct (value_is_true_or_false cond_value) as [Eq|Ne].
+      {
+        used_value f fr pc i vt vt_value Hvt Hvt_reg.
+        generalize (eval_select_true
+          p stk h fr f pc dst t next cond vt vf
+          cond_value vt_value Hexec Hcond Hvt Eq
+        ); step_state.
+      }
+      {
+        used_value f fr pc i vf vf_value Hvf Hvf_reg.
+        generalize (eval_select_false
+          p stk h fr f pc dst t next cond vt vf
+          cond_value vf_value Hexec Hcond Hvf Ne
+        ); step_state.
+      }
+    }
+    {
+      generalize (eval_frame
+        p stk h fr f pc dst next object offset
+        Hexec
+      ); step_state.
+    }
+    {
+      generalize (eval_global
+        p stk h fr f pc dst next segment object offset
+        Hexec
+      ); step_state.
+    }
+    { generalize (eval_func p stk h fr f pc dst next func Hexec); step_state. }
+    { generalize (eval_und p stk h fr f pc t dst next Hexec); step_state. }
+    {
+      used_value f fr pc i arg arg_value Harg Harg_reg.
+      inversion Hwti; subst t0 dst0 next0 op0 arg0.
+      unfold well_typed_reg in ARG_TY;
+      destruct (VALS arg arg_value Harg) as [arg_ty [Harg_ty Harg_type_of]];
+      rewrite ARG_TY in Harg_ty; inversion Harg_ty; subst argt.
+      destruct (unary_value_or_signal op arg_value arg_ty t OP Harg_type_of) as
+        [ [dst_value [_ Hdst]]
+        | [sig Hsig]
+        ].
+      {
+        generalize (eval_unary_value
+          p stk h fr f pc dst t next op arg dst_value arg_value
+          Hexec Harg Hdst
+        ); step_state.
+      }
+      {
+        generalize (eval_unary_signal
+          p stk h fr f pc dst t next op arg arg_value sig
+          Hexec Harg Hsig
+        ); step_state.
+      }
+    }
+    {
+      used_value f fr pc i lhs lhs_value Hlhs Hlhs_reg.
+      used_value f fr pc i rhs rhs_value Hrhs Hrhs_reg.
+      inversion Hwti; subst t0 dst0 next0 op0 l r.
+      unfold well_typed_reg in LHS_TY;
+      destruct (VALS lhs lhs_value Hlhs) as [lhs_ty [Hlhs_ty Hlhs_type_of]];
+      rewrite LHS_TY in Hlhs_ty; inversion Hlhs_ty; subst tl.
+      unfold well_typed_reg in RHS_TY;
+      destruct (VALS rhs rhs_value Hrhs) as [rhs_ty [Hrhs_ty Hrhs_type_of]];
+      rewrite RHS_TY in Hrhs_ty; inversion Hrhs_ty; subst tr.
+      destruct (binary_value_or_signal
+        op lhs_value rhs_value lhs_ty rhs_ty t
+        OP Hlhs_type_of Hrhs_type_of) as [[dst_value [_ Hdst]]|[sig Hsig]].
+      {
+        generalize (eval_binary_value
+          p stk h fr f pc dst t op lhs rhs next lhs_value rhs_value dst_value
+          Hexec Hlhs Hrhs Hdst
+        ); step_state.
+      }
+      {
+        generalize (eval_binary_signal
+          p stk h fr f pc dst t op lhs rhs next lhs_value rhs_value sig
+          Hexec Hlhs Hrhs Hsig
+        ); step_state.
+      }
+    }
+    {
+      used_value f fr pc i src src_value Hsrc Hsrc_reg.
+      generalize (eval_mov
+        p stk h fr f pc dst t next src src_value
+        Hexec Hsrc
+      ); step_state.
+    }
+    {
+      used_value f fr pc i sno sno_value Hsno Hsno_reg.
+      symmetry in Hsno_reg.
+      generalize (VALS sno sno_value Hsno_reg); intros [ty [Hty Hty_of]].
+      inversion Hwti; subst next0 dst0 sno0 args0.
+      unfold well_typed_reg in SNO_TY.
+      rewrite <- Hty in SNO_TY; inversion SNO_TY; subst ty.
+      assert (Hargs_live: forall arg, In arg args -> LiveAt f arg (fr_pc fr)).
+      {
+        intros arg Hin'.
+        apply live_at with (use := pc) (p := [pc]).
+        - subst pc; constructor; apply REACH.
+        - intros def contra Hin; inversion Hin; subst; contradiction.
+        - apply used_at_inst; apply inst_used_at with i; subst; try constructor; auto.
+      }
+      generalize (syscall_args
+        p f fr args (ty_env f)
+        FUNC ARG_TY REGS Hargs_live VALS
+      ); intros [sys_values Hsys_args].
+      destruct (syscall_number_complete sno_value Hty_of) as [[s Esys]|[ENoSys|EUnd]].
+      {
+        destruct (syscall_ret_or_sig s sys_values stk h) as
+          [ [tr [stk'' [h'' [dst_value Eret]]]]
+          | [sig [tr Esig]]
+          ].
+        {
+          generalize (eval_syscall_ret
+            p stk h fr f pc dst next tr args sys_values sno s sno_value
+            dst_value stk'' h''
+            Hsys_args Hsno_reg Esys Hexec Eret
+          ); step_state.
+        }
+        {
+          generalize (eval_syscall_sig
+            p stk h fr f pc dst next tr args sys_values sno s sno_value sig
+            Hsys_args Hsno_reg Esys Hexec Esig
+          ); step_state.
+        }
+      }
+      {
+        generalize (eval_syscall_nosys
+          p stk h fr f pc dst next [] args sys_values sno sno_value
+          Hsys_args Hsno_reg ENoSys Hexec
+        ); step_state.
+      }
+      {
+        generalize (eval_syscall_und_enosys
+          p stk h fr f pc dst next [] args sys_values sno sno_value
+        ); step_state.
+      }
+    }
+    {
+      used_value f fr pc i callee callee_value Hcallee Hcallee_reg.
+      used_callee h callee callee_value Hcallee_reg args0.
+      used_args pc i args values Hvalues.
+      inversion Eq as [func Hfunc]; subst callee_value.
+      generalize (FN_VALS callee func Hcallee); intros Hsome_func.
+      destruct (p ! func) as [callee_fn|] eqn:Efunc; try contradiction.
+      symmetry in Efunc.
+      generalize (eval_call
+        p stk h stk_fr stk_frs stk_next stk_frames stk_init
+        fr f pc callee next dst func callee_fn args values
+        Hexec Hcallee Efunc Hvalues
+      ); rewrite Hstk; step_state.
+    }
+    {
+      used_value f fr pc i callee callee_value Hcallee Hcallee_reg.
+      used_callee h callee callee_value Hcallee_reg args.
+      used_args pc i args values Hvalues.
+      inversion Eq as [func Hfunc]; subst callee_value.
+      generalize (FN_VALS callee func Hcallee); intros Hsome_func.
+      destruct (p ! func) as [callee_fn|] eqn:Efunc; try contradiction.
+      symmetry in Efunc.
+      generalize (eval_invoke
+        p stk h stk_fr stk_frs stk_next stk_frames stk_init
+        fr f pc callee next dst exn func callee_fn args values
+        Hexec Hcallee Efunc Hvalues
+      ); rewrite Hstk; step_state.
+    }
+    {
+      used_value f fr pc i callee callee_value Hcallee Hcallee_reg.
+      used_callee h callee callee_value Hcallee_reg args.
+      used_args pc i args values Hvalues.
+      inversion Eq as [fn Hfn]. rewrite <- Hfn in Hcallee.
+      generalize (FN_VALS callee fn Hcallee); intros Hfn_not_none.
+      destruct (p ! fn) as [func|] eqn:Efunc; try contradiction.
+      symmetry in Efunc.
+      generalize (eval_tcall
+        p stk h stk_fr stk_frs stk_next stk_frames stk_init fr f
+        pc callee fn func args values Hexec Hcallee Efunc Hvalues).
+      rewrite Hstk.
+      step_state.
+    }
+    {
+      used_value f fr pc i callee callee_value Hcallee Hcallee_reg.
+      used_callee h callee callee_value Hcallee_reg args.
+      used_args pc i args values Hvalues.
+      inversion Eq as [fn Hfn]. rewrite <- Hfn in Hcallee.
+      generalize (FN_VALS callee fn Hcallee); intros Hfn_not_none.
+      destruct (p ! fn) as [func|] eqn:Efunc; try contradiction.
+      symmetry in Efunc.
+      generalize (eval_tinvoke
+        p stk h stk_fr stk_frs stk_next stk_frames stk_init fr f
+        pc callee exn fn func args values Hexec Hcallee Efunc Hvalues).
+      rewrite Hstk.
+      step_state.
+    }
+    {
+      used_value f fr pc i addr addr_value Haddr Haddr_reg.
+      used_value f fr pc i value value_value Hvalue Hvalue_reg.
+      destruct (store_value_signal_break stk h addr_value value_value) as
+        [ [h'' Evalue]
+        | [ [s Esig]| Ebreak]
+        ].
+      {
+        generalize (eval_st_value
+          p stk h fr f pc next addr value addr_value value_value h''
+          Hexec Haddr Hvalue Evalue
+        ); step_state.
+      }
+      {
+        generalize (eval_st_sig
+          p stk h fr f pc next addr value addr_value s
+          Hexec Haddr Esig
+        ); step_state.
+      }
+      {
+        generalize (eval_st_break
+          p stk h fr f pc next addr value addr_value
+          Hexec Haddr Ebreak
+        ); step_state.
+      }
+    }
+    {
+      destruct (top_or_return stk) as [Htop|[vr [vrs Hret]]].
+      {
+        generalize (eval_ret_top p stk h fr f pc value Hexec Htop); step_state.
+      }
+      {
+        inversion Hret as [next frames init top ret frs H']; subst ret frs.
+        rewrite <- Hstk in H'; inversion H'; subst top frames init next.
+        assert (Hmvr: In vr stk_frs). { subst; left; auto. }
+        generalize (Hvalid_mid vr Hmvr); intros Hmid.
+        inversion Hmid. subst p0 fr_id frames.
+        rewrite H'; rewrite Hstk.
+        assert (Hret_addr: exists (ret_pc: node), ReturnAddress i1 ret_pc).
+        {
+           destruct RETURN as [H''|[tr [dstr H'']]];
+           inversion H''; exists next; constructor.
+        }
+        destruct Hret_addr as [ret_pc Hret_pc].
+        assert (Hret_to_frame: ReturnToFrame p stk vr vrs i1 ret_pc).
+        {
+          subst stk stk_frs; apply return_to_frame with fr0 f0; auto.
+        }
+        destruct RETURN as [Hvoid|[tr [dstr Hcall]]].
+        {
+          generalize (eval_ret_void
+            p stk h fr f pc value vrs i1 vr ret_pc
+            Hexec Hret_to_frame Hvoid
+          ); step_state.
+        }
+        {
+          assert (Hrv: exists v, ReturnValue fr value tr v).
+          {
+            destruct value as [arg|] eqn:Evalue.
+            {
+              used_value f fr pc i arg arg_value Harg Harg_reg.
+              destruct (TypeOfValue_dec arg_value tr).
+              { exists arg_value; constructor; auto. }
+              { exists VUnd; apply return_some_und with arg_value; auto. }
+            }
+            {
+              exists VUnd; constructor.
+            }
+          }
+          destruct Hrv as [ret_value Hret_value].
+          generalize (eval_ret_value
+            p stk h fr f pc value vrs i1 vr tr dstr ret_pc ret_value
+            Hexec Hret_to_frame Hcall Hret_value
+          ); step_state.
+        }
+      }
+    }
+    {
+      used_value f fr pc i cond cond_value Hcond Hcond_reg.
+      destruct (value_is_true_or_false cond_value) as [Et|Ef].
+      {
+        generalize (eval_jcc_true
+          p stk h fr f pc cond bt bf cond_value
+          Hexec Hcond Et
+        ); step_state.
+      }
+      {
+        generalize (eval_jcc_false
+          p stk h fr f pc cond bt bf cond_value
+          Hexec Hcond Ef
+        ); step_state.
+      }
+    }
+    {
+      generalize (eval_jmp p stk h fr f pc target); step_state.
+    }
+    {
+      generalize (eval_trap p stk h fr f pc Hexec); step_state.
+    }
+  }
+  { inversion Hv. }
+  { inversion Hv. }
+  { inversion Hv. }
+Qed.
+
