SmallStep_Valid.v
@@ -1,0 +1,85 @@
+(* This file is part of the LLIR Semantics project. *)
+(* Licensing information is available in the LICENSE file. *)
+(* (C) 2020 Nandor Licker. All rights reserved. *)
+
+Require Import Coq.Lists.List.
+Require Import Coq.ZArith.ZArith.
+
+Require Import LLIR.Values.
+Require Import LLIR.Maps.
+Require Import LLIR.LLIR.
+Require Import LLIR.Dom.
+Require Import LLIR.Eval.
+Require Import LLIR.SSA.
+Require Import LLIR.Block.
+Require Import LLIR.Typing.
+Require Import LLIR.Signal.
+Require Import LLIR.Liveness.
+Require Import LLIR.Syscall.
+Require Import LLIR.Frame.
+Require Import LLIR.State.
+Require Import LLIR.SmallStep.
+
+Import ListNotations.
+
+
+
+Theorem small_step_valid:
+  forall (p: prog) (st: estate) (st': estate) (tr: trace),
+    WellTypedProg p ->
+    valid_prog p ->
+    Normal p st ->
+    step p st tr st' ->
+    ~Final st' ->
+    Normal p st'.
+(*
+Proof.
+  intros p st st' tr Hwt Hvp Hnormal Hstep Hnf;
+    inversion Hnormal; clear Hnormal; subst p0;
+    inversion Hstep; clear Hstep; subst tr;
+    inversion EXEC; inversion FR; inversion VALID;
+    subst p0 p1 p2 fr2 frames1 fr_id1 f0 fr0;
+    try (
+      rewrite <- H in H0; rewrite <- H3 in H0; inversion H0; clear H0;
+      subst h0 init0 frames0 next1 frs0 fr_id0;
+      rewrite <- FRAME in FRAME0; inversion FRAME0; clear FRAME0; subst fr1;
+      rewrite <- FUNC in FUNC0; inversion FUNC0; clear FUNC0; subst f1
+    );
+    (
+      assert (Hvalid_func: valid_func f);
+      [ unfold valid_prog in Hvp; apply Hvp with (fr_func fr); auto |]
+    );
+    try match goal with
+    | [ H: context [ stk_set_pc _ ?next ] |- _ ] => 
+      assert (Hsucc: SuccOf f pc next);
+        [ apply ((fn_succs_are_valid f Hvalid_func) pc next i); 
+          subst;
+          auto;
+          constructor 
+        |]
+    end;
+    subst pc.
+  {
+    destruct ((fn_insts f) ! next0) as [inext|] eqn:Einext; [|contradiction].
+    constructor; auto.
+    {
+      apply valid_top_frame with (fr := set_pc fr next0).
+      {
+        rewrite PTrie.update_eq; simpl.
+        rewrite <- FRAME; simpl.
+        reflexivity.
+      }
+      {
+        apply valid_frame with f inext; 
+        unfold stk_set_pc; unfold set_pc; simpl; auto.
+        apply reach_succ with (a := fr_pc fr); auto.
+        intros r Hlive.
+        
+      }
+    }
+    {
+    }
+  }
+Qed.
+*)
+Admitted.
